Changed value semantics embedding of word arrays
The new embedding of word arrays in the value semantics now contains the
type of the elements in the word array. The main benefit of this change
is that it removes duplication of abstractions for word array function,
due to different word sizes, which was previously thought to be
necessary. This then makes creating a tactic for proving scorres easier
since the same tactic will work even for the different word sizes
(assuming the correct lemmas and definitions are added the simpset).

Other changes were fixes to the definitions and proofs to reflect the
change of embedding of word arrays.

cogent/examples/wa_connect/WordArray_Abstractions.thy
@@ -27,6 +27,23 @@ lemma word_mult_cancel_left:
    apply fastforce
    done
 
+fun is_prim_type :: "type \<Rightarrow> bool"
+  where
+"is_prim_type (TPrim _) = True" |
+"is_prim_type _ = False"
+
+fun is_num_type :: "prim_type \<Rightarrow> bool"
+  where
+"is_num_type (Num _) = True" |
+"is_num_type _ = False"
+
+fun size_of_num_type :: "num_type \<Rightarrow> ptrtyp"
+  where
+"size_of_num_type U8 = 1" |
+"size_of_num_type U16 = 2" |
+"size_of_num_type U32 = 4" |
+"size_of_num_type U64 = 8"
+
 section "WordArray Locale Definition"
 
 locale WordArray = main_pp_inferred begin
@@ -44,7 +61,10 @@ locale WordArray = main_pp_inferred begin
 
   definition "abs_typing_v a name \<tau>s \<equiv>
     (case a of
-      VWA xs \<Rightarrow> name = ''WordArray'' \<and> \<tau>s = [TPrim (Num U32)] \<and> (\<forall>i < length xs. \<exists>x. xs ! i = VPrim (LU32 x))
+      VWA (TPrim (Num U8)) xs \<Rightarrow> name = ''WordArray'' \<and> \<tau>s = [TPrim (Num U8)] \<and> (\<forall>i < length xs. \<exists>x. xs ! i = VPrim (LU8 x))
+    | VWA (TPrim (Num U16)) xs \<Rightarrow> name = ''WordArray'' \<and> \<tau>s = [TPrim (Num U16)] \<and> (\<forall>i < length xs. \<exists>x. xs ! i = VPrim (LU16 x))
+    | VWA (TPrim (Num U32)) xs \<Rightarrow> name = ''WordArray'' \<and> \<tau>s = [TPrim (Num U32)] \<and> (\<forall>i < length xs. \<exists>x. xs ! i = VPrim (LU32 x))
+    | VWA (TPrim (Num U64)) xs \<Rightarrow> name = ''WordArray'' \<and> \<tau>s = [TPrim (Num U64)] \<and> (\<forall>i < length xs. \<exists>x. xs ! i = VPrim (LU64 x))
     | _ \<Rightarrow> name = ''Unknown Abstract Type'' \<and> \<tau>s = [])"
 
   definition  "abs_upd_val' au av name \<tau>s sig (r :: ptrtyp set) (w :: ptrtyp set) \<sigma> \<equiv>
@@ -52,7 +72,7 @@ locale WordArray = main_pp_inferred begin
     (case au of
       WAU32 len arr \<Rightarrow>
         (case av of 
-          VWA xs \<Rightarrow> unat len = length xs \<and> 
+          VWA (TPrim (Num U32)) xs \<Rightarrow> unat len = length xs \<and> 
                       (\<forall>i < len. \<exists>x. \<sigma>(arr + 4 * i) = option.Some (UPrim (LU32 x)) \<and> 
                                      xs ! (unat i) = VPrim (LU32 x))
           | _ \<Rightarrow> False)
@@ -83,6 +103,7 @@ section "Sublocale Proof"
 sublocale WordArray \<subseteq> Generated_cogent_shallow _ abs_repr_u abs_typing_v abs_typing_u abs_upd_val'
   apply (unfold abs_repr_u_def[abs_def] abs_typing_v_def[abs_def] abs_typing_u_def[abs_def] abs_upd_val'_def[abs_def])
   apply (unfold_locales; clarsimp split: vatyp.splits atyp.splits)
+           apply (case_tac x11; clarsimp; case_tac x5; clarsimp; case_tac x1; clarsimp)
           apply (case_tac s; clarsimp; case_tac x11a; clarsimp)
          apply (case_tac s; clarsimp; case_tac x11a; clarsimp)
         apply (case_tac s; clarsimp; case_tac x11a; clarsimp)
@@ -95,15 +116,17 @@ sublocale WordArray \<subseteq> Generated_cogent_shallow _ abs_repr_u abs_typing
     apply (rule_tac x = x in exI)
     apply (case_tac s; clarsimp; case_tac x11a; clarsimp;
            drule_tac x = "x12 + 4 * i" in orthD1; simp; rule_tac x = i in exI; simp)
-   apply (case_tac s; clarsimp; case_tac x11a; clarsimp)
-  apply (case_tac s; clarsimp; case_tac x11a; clarsimp)
-   apply (rule conjI; clarsimp; erule_tac x = "x12 + 4 * i" in allE; clarsimp)
+   apply (case_tac x11; clarsimp; case_tac x5; clarsimp; case_tac x1; clarsimp)
+   apply (case_tac s; clarsimp; case_tac x11; clarsimp)
+  apply (case_tac x11; clarsimp; case_tac x5; clarsimp; case_tac x1; clarsimp)
+  apply (case_tac s; clarsimp; case_tac x11; clarsimp)
+   apply (rule conjI; clarsimp; erule_tac x = "x12b + 4 * i" in allE; clarsimp)
     apply (erule_tac x = i in allE; clarsimp)
     apply (rule_tac x = x in exI)
     apply auto[1]
    apply (erule_tac x = i in allE; clarsimp)
    apply auto[1]
-  apply (rule conjI; clarsimp; erule_tac x = "x12 + 4 * i" in allE; clarsimp)
+  apply (rule conjI; clarsimp; erule_tac x = "x12b + 4 * i" in allE; clarsimp)
     apply (erule_tac x = i in allE; clarsimp)
     apply (rule_tac x = x in exI)
     apply auto[1]
@@ -134,21 +157,13 @@ lemma take_drop_Suc:
 *)
 
 subsection "Shallow Word Array Value Relation"
-(*
-overloading
-  valRel_WordArrayBool \<equiv> valRel
-begin
-  definition valRel_WordArrayBool: 
-    "\<And>\<xi> x v. valRel_WordArrayBool (\<xi> :: (funtyp,vabstyp) vabsfuns) (x :: bool WordArray) (v :: (funtyp, vabstyp) vval) \<equiv> 
-      \<exists>xs. v = VAbstract (VWA xs) \<and> length x = length xs \<and> (\<forall>i < length xs. xs ! i = VPrim (LBool (x ! i)))"
-end
 
 overloading
   valRel_WordArrayU8 \<equiv> valRel
 begin
   definition valRel_WordArrayU8: 
     "\<And>\<xi> x v. valRel_WordArrayU8 (\<xi> :: (funtyp,vabstyp) vabsfuns) (x :: (8 word) WordArray) (v :: (funtyp, vabstyp) vval) \<equiv> 
-      \<exists>xs. v = VAbstract (VWA xs) \<and> length x = length xs \<and> (\<forall>i < length xs. xs ! i = VPrim (LU8 (x ! i)))"
+      \<exists>xs. v = VAbstract (VWA (TPrim (Num U8)) xs) \<and> length x = length xs \<and> (\<forall>i < length xs. xs ! i = VPrim (LU8 (x ! i)))"
 end
 
 overloading
@@ -156,25 +171,27 @@ overloading
 begin
   definition valRel_WordArrayU16: 
     "\<And>\<xi> x v. valRel_WordArrayU16 (\<xi> :: (funtyp,vabstyp) vabsfuns) (x :: (16 word) WordArray) (v :: (funtyp, vabstyp) vval) \<equiv> 
-      \<exists>xs. v = VAbstract (VWA xs) \<and> length x = length xs \<and> (\<forall>i < length xs. xs ! i = VPrim (LU16 (x ! i)))"
+      \<exists>xs. v = VAbstract (VWA (TPrim (Num U16)) xs) \<and> length x = length xs \<and> (\<forall>i < length xs. xs ! i = VPrim (LU16 (x ! i)))"
 end
-*)
+
 overloading
   valRel_WordArrayU32 \<equiv> valRel
 begin
   definition valRel_WordArrayU32: 
     "\<And>\<xi> x v. valRel_WordArrayU32 (\<xi> :: (funtyp,vabstyp) vabsfuns) (x :: (32 word) WordArray) (v :: (funtyp, vabstyp) vval) \<equiv> 
-      \<exists>xs. v = VAbstract (VWA xs) \<and> length x = length xs \<and> (\<forall>i < length xs. xs ! i = VPrim (LU32 (x ! i)))"
+      \<exists>xs. v = VAbstract (VWA (TPrim (Num U32)) xs) \<and> length x = length xs \<and> (\<forall>i < length xs. xs ! i = VPrim (LU32 (x ! i)))"
 end
-(*
+
 overloading
   valRel_WordArrayU64 \<equiv> valRel
 begin
   definition valRel_WordArrayU64: 
     "\<And>\<xi> x v. valRel_WordArrayU64 (\<xi> :: (funtyp,vabstyp) vabsfuns) (x :: (64 word) WordArray) (v :: (funtyp, vabstyp) vval) \<equiv> 
-      \<exists>xs. v = VAbstract (VWA xs) \<and> length x = length xs \<and> (\<forall>i < length xs. xs ! i = VPrim (LU64 (x ! i)))"
+      \<exists>xs. v = VAbstract (VWA (TPrim (Num U64)) xs) \<and> length x = length xs \<and> (\<forall>i < length xs. xs ! i = VPrim (LU64 (x ! i)))"
 end
-*)
+
+
+
 subsection "Shallow Word Array Function Definitions"
 
 overloading
@@ -195,8 +212,9 @@ overloading
   wordarray_get' \<equiv> wordarray_get
 begin
 definition wordarray_get':
- "wordarray_get' (x :: (32 word WordArray, 32 word) RR) \<equiv> (if unat (RR.p2\<^sub>f x) < length (RR.p1\<^sub>f x) then (RR.p1\<^sub>f x) ! unat (RR.p2\<^sub>f x) else 0)" 
+ "wordarray_get' (x :: (('a::len8) word WordArray, 32 word) RR) \<equiv> (if unat (RR.p2\<^sub>f x) < length (RR.p1\<^sub>f x) then (RR.p1\<^sub>f x) ! unat (RR.p2\<^sub>f x) else 0)" 
 end
+
 
 overloading
   wordarray_fold_no_break' \<equiv> wordarray_fold_no_break
@@ -259,39 +277,40 @@ subsubsection "Value Semantics"
     @{term "VWA xs"} means we cannot determine what word array it is meant to represent in the case
     that @{term "xs::(funtyp, vabstyp) vval list"} is empty. Either we need to define a new dataype
     or we modify the current type to include the word type. \<close>
-definition val_wa_length_0
+definition val_wa_length
   where
-  "val_wa_length_0 x y = (\<exists>xs len. x = VAbstract (VWA xs) \<and> y = VPrim (LU32 len) \<and> 
-                                length xs = unat len)" 
+  "val_wa_length x y = (\<exists>xs len ts. x = VAbstract (VWA (TPrim ts) xs) \<and> y = VPrim (LU32 len) \<and> 
+                          is_num_type ts \<and> length xs = unat len)" 
 
-
-definition val_wa_get_0
+definition val_wa_get
   where
-  "val_wa_get_0 x y =
-      (\<exists>xs idx v. x = VRecord [VAbstract (VWA xs), VPrim (LU32 idx)] \<and> y = VPrim (LU32 v) \<and>
-       (unat idx < length xs \<longrightarrow> xs ! unat idx = y) \<and> (\<not> unat idx < length xs \<longrightarrow> v = 0))" 
+  "val_wa_get x y =
+      (\<exists>xs ts idx v. x = VRecord [VAbstract (VWA (TPrim ts) xs), VPrim (LU32 idx)] \<and> is_num_type ts \<and>
+       y = VPrim v \<and> lit_type v = ts \<and> (unat idx < length xs \<longrightarrow> xs ! unat idx = y) \<and> 
+       (\<not> unat idx < length xs \<longrightarrow> (v = LU8 0 \<or> v = LU16 0 \<or> v = LU32 0 \<or> v = LU64 0)))" 
 
-definition val_wa_put2_0
+definition val_wa_put2
   where
-  "val_wa_put2_0 x y =
-      (\<exists>xs idx val. x = VRecord [VAbstract (VWA xs), VPrim (LU32 idx), VPrim (LU32 val)] \<and>
-       y = VAbstract (VWA (xs[unat idx := VPrim (LU32 val)])))" 
+  "val_wa_put2 x y =
+      (\<exists>xs ts idx val. x = VRecord [VAbstract (VWA (TPrim ts) xs), VPrim (LU32 idx), VPrim val] \<and>
+       is_num_type ts \<and> lit_type val = ts \<and>
+       y = VAbstract (VWA (TPrim ts) (xs[unat idx := VPrim val])))" 
 
 
 fun \<xi>m :: "(char list, vatyp) vabsfuns" 
   where
   "\<xi>m x y z = 
-    (if x = ''wordarray_put2_0'' then val_wa_put2_0 y z
-     else (if x = ''wordarray_get_0'' then val_wa_get_0 y z
-           else (if x = ''wordarray_length_0'' then val_wa_length_0 y z
+    (if x = ''wordarray_put2_0'' then val_wa_put2 y z
+     else (if x = ''wordarray_get_0'' then val_wa_get y z
+           else (if x = ''wordarray_length_0'' then val_wa_length y z
                  else False)))" 
 
 fun \<xi>p :: "(char list, vatyp) vabsfuns" 
   where
   "\<xi>p x y z = 
-    (if x = ''wordarray_put2'' then val_wa_put2_0 y z
-     else (if x = ''wordarray_get'' then val_wa_get_0 y z
-           else (if x = ''wordarray_length'' then val_wa_length_0 y z
+    (if x = ''wordarray_put2'' then val_wa_put2 y z
+     else (if x = ''wordarray_get'' then val_wa_get y z
+           else (if x = ''wordarray_length'' then val_wa_length y z
                  else False)))" 
 
 subsection "Level 1 \<xi> Abstractions"
@@ -1263,7 +1282,7 @@ lemma val_wa_foldnb_bod_0p_back_step:
 definition val_wa_foldnb_0
   where
   "val_wa_foldnb_0 x y = (\<exists>xs frm to acc r func. 
-      x = VRecord [VAbstract (VWA xs), VPrim (LU32 frm), VPrim (LU32 to), func, VPrim (LU32 acc),
+      x = VRecord [VAbstract (VWA (TPrim (Num U32)) xs), VPrim (LU32 frm), VPrim (LU32 to), func, VPrim (LU32 acc),
                    VUnit] \<and> y = VPrim (LU32 r) \<and> (\<forall>i < length xs. \<exists>v. xs ! i = VPrim (LU32 v)) \<and>
       (case func of
             VFunction f ts \<Rightarrow> (\<Xi>, [], [option.Some abbreviatedType1] \<turnstile> (App (Fun f ts) (Var 0)) : 
@@ -1280,7 +1299,7 @@ definition val_wa_foldnb_0
 
 definition val_wa_foldnb_0p
   where
-  "val_wa_foldnb_0p x y = (\<exists>fs xs frm to. x = VRecord fs \<and> fs! 0 = VAbstract (VWA xs) \<and>
+  "val_wa_foldnb_0p x y = (\<exists>fs xs frm to. x = VRecord fs \<and> fs! 0 = VAbstract (VWA (TPrim (Num U32)) xs) \<and>
       fs ! 1 = VPrim (LU32 frm) \<and> fs ! 2 = VPrim (LU32 to) \<and> length fs = 6 \<and> 
       (case fs ! 3 of
             VFunction f ts \<Rightarrow> val_wa_foldnb_bod_0p xs (unat frm) (unat to)
